aarch64 aspec+ainvs: make pt_walk_is_aligned true
On RISCV64, we had the nice property that pt_walk can only produce
aligned addresses. This alignment is important for further address
computation.

It turns out that the same is true on AARCH64, because the bottom 12
bits of page table addresses are not stored in PTEs. PagePTEs can only
point to normal page tables, so there is not variation in the size of
the alignment.

This commit uses a similar encoding to RISCV64 to achieve this pt_walk
property without using an additional invariant.

Signed-off-by: Gerwin Klein <gerwin.klein@proofcraft.systems>

spec/abstract/AARCH64/Arch_Structs_A.thy
@@ -15,6 +15,10 @@ imports
   ExecSpec.Kernel_Config_Lemmas
 begin
 
+context begin interpretation Arch .
+lemmas [code] = pageBits_def ipa_size_def
+end
+
 context Arch begin global_naming AARCH64_A
 
 text \<open>
@@ -65,16 +69,44 @@ subsection \<open>Page tables\<close>
 datatype vm_attribute = Global | Execute | Device
 type_synonym vm_attributes = "vm_attribute set"
 
+text \<open>
+  The C field @{text base_addr} for next-level tables of @{text PagePTE}s is a 36 bit field-high
+  value, i.e., a 48-bit word with the bottom 12 bits always set to 0. (They must be 0 due to
+  alignment). Since Arm does not specify a name, we are re-using the RISC-V name @{text ppn}
+  (physical page number) for the concept of encoding only the significant bits of this address.
+
+  In addition to the bottom 12 bits being 0 (where 12 = @{const pageBits}), we also know that
+  the base address of the next level table is a physical address and therefore has the same width
+  as intermediate physical addresses (@{const ipa_size}). We can therefore be more precise in the
+  encoding here: the significant bits of the next-level page table address go from @{const ipa_size}
+  at the top to @{const pageBits} at the bottom. Similar to the ppn on RISC-V we store a word
+  of that size, and shift by @{const pageBits} to get the address. This encodes both a size invariant
+  and an alignment invariant in the type, which functions like @{text pt_walk} rely on.
+
+  To provide the same field name as in C, we define @{text pte_base_addr} as the main accessor
+  function.\<close>
+value_type ppn_len = "ipa_size - pageBits"
+type_synonym ppn = "ppn_len word"
+
 datatype pte =
     InvalidPTE
   | PagePTE
-      (pte_base_addr : paddr)
+      (pte_page_addr : paddr)
       (pte_is_small_page : bool)
       (pte_attr : vm_attributes)
       (pte_rights : vm_rights)
   | PageTablePTE
-      (pte_base_addr : paddr)
+      (pte_ppn : ppn)
 
+definition paddr_from_ppn :: "ppn \<Rightarrow> paddr" where
+  "paddr_from_ppn addr \<equiv> ucast addr << pageBits"
+
+definition pte_base_addr :: "pte \<Rightarrow> paddr" where
+  "pte_base_addr pte \<equiv>
+    if is_PageTablePTE pte then paddr_from_ppn (pte_ppn pte) else pte_page_addr pte"
+
+definition ppn_from_pptr :: "obj_ref \<Rightarrow> ppn" where
+  "ppn_from_pptr p = ucast (addrFromPPtr p >> pageBits)"
 
 definition vs_index_bits :: nat where
   "vs_index_bits \<equiv> if config_ARM_PA_SIZE_BITS_40 then 10 else (9::nat)"
@@ -207,6 +239,12 @@ definition table_size :: "pt_type \<Rightarrow> nat" where
 
 definition pt_bits :: "pt_type \<Rightarrow> nat" where
   "pt_bits pt_t \<equiv> table_size pt_t"
+
+(* sanity check *)
+lemma ppn_len:
+  "LENGTH(ppn_len) = ipa_size - pt_bits NormalPT_T"
+  by (simp add: pt_bits_def table_size_def ptTranslationBits_def pte_bits_def word_size_bits_def
+                ipa_size_def Kernel_Config.config_ARM_PA_SIZE_BITS_40_def)
 
 primrec arch_obj_size :: "arch_cap \<Rightarrow> nat" where
   "arch_obj_size (ASIDPoolCap _ _) = pageBits"
