spec/abstract/AARCH64/Init_A.thy
@@ -28,9 +28,6 @@ definition arm_global_pt_ptr :: obj_ref where
 definition init_irq_node_ptr :: obj_ref where
   "init_irq_node_ptr = pptr_base + 0x3000"
 
-definition ipa_size :: nat where
-  "ipa_size \<equiv> if config_ARM_PA_SIZE_BITS_40 then 40 else 44"
-
 (* The highest user-virtual address that is still canonical.
    It can be larger than user_vtop, which is the highest address we allow to be mapped.
    For AArch64-hyp, user-virtual addresses are IPAs and since there is no sign extension,
